adapt nj1.v to monad approach

nj1.v
@@ -2,151 +2,52 @@
 
 Require Import Lia.
 Require Import stdlib_more.
-Require Export fot.
+Require Export foformulas.
 
 Set Implicit Arguments.
 
 
-(** * Formulas and Proofs *)
+(** * Proofs *)
 
-Section Formulas.
+Section Proofs.
 
-Context { vatom : DecType } { tatom : Type }.
-Notation term := (@term vatom tatom).
-Notation closed t := (freevars t = nil).
-Notation tup := (@tup vatom tatom).
+Context { vatom : DecType } { tatom fatom : Type }.
+Inductive Ncon := .
+Inductive Bcon := imp_con.
+Inductive Qcon := frl_con | exs_con.
 
-Hint Rewrite
-  (@tup_tup_com vatom tatom) (@tup_tsubs_com vatom tatom)
-  (@ntsubs_tup_com vatom tatom) (@ntsubs_z_tup vatom tatom)
-  (@freevars_tup vatom tatom) (@tsubs_tsubs_eq vatom tatom) : term_db.
-Hint Resolve (@closed_nofreevars vatom tatom) : term_db.
-Hint Rewrite (@freevars_ntsubs vatom tatom) using intuition; fail : term_db.
-Hint Rewrite (@nfree_tsubs vatom tatom)
-  using try (intuition; fail); (try apply closed_nofreevars); intuition; fail : term_db.
-Hint Rewrite (@ntsubs_tsubs_com vatom tatom)
-  using try (intuition; fail); (try apply closed_nofreevars); intuition; fail : term_db.
-Hint Rewrite (@tsubs_tsubs_com vatom tatom)
-  using try (intuition; fail); (try apply closed_nofreevars); intuition; fail : term_db.
-Hint Rewrite (@freevars_tsubs_closed vatom tatom)
-  using intuition; fail : term_db.
+Arguments tvar {_} {_} {T} _.
 
-Context { fatom : Type }.  (* relation symbols for [formula] *)
+Notation term := (@term vatom tatom nat).
+Notation closed t := (tvars t = nil).
+Notation fclosed r := (forall n, closed (r n)).
+Notation "↑ r" := (fdblift r) (at level 25, format "↑ r").
+Notation "v // ↓ k" := (fdbsubs k v) (at level 18, format "v // ↓ k").
+Notation "A ⟦ r ⟧" := (dbsubs r A) (at level 8, left associativity, format "A ⟦ r ⟧").
+Notation "A [ u // x ]" := (subs x u A) (at level 8, format "A [ u // x ]").
+Notation "⇑" := fup.
+Notation "A ↑" := (A⟦⇑⟧) (at level 8, format "A ↑").
+Notation "x ∈ A" := (In x (freevars A)) (at level 30).
 
-(** formulas *)
-(** first-order formulas in the langage: implication, universal quantification *)
-Inductive formula :=
-| var : fatom -> list term -> formula
-| imp : formula -> formula -> formula
-| frl : vatom -> formula -> formula
-| exs : vatom -> formula -> formula.
-(* alternative representation (thanks D. Pous)
-Inductive qtf := Frl | Exs.  (* use bool *)
-Inductive qformula :=
-| qvar : fatom -> list term -> qformula
-| qimp : qformula -> qformula -> qformula
-| qant : qtf -> vatom -> qformula -> qformula.
-Notation qfrl := (qant Frl).
-Notation qexs := (qant Exs).
-(* could be generalized to a family of binary connectives,
-   a family of unary connectives, etc
-*)
-*)
+Notation formula := (@formula vatom tatom fatom Ncon Bcon Qcon nat).
+Notation fvar := (@fvar vatom tatom fatom Ncon Bcon Qcon nat).
+Notation imp := (fbin imp_con).
+Notation frl := (fqtf frl_con).
+Notation exs := (fqtf exs_con).
 
-Ltac formula_induction A :=
-  (try intros until A) ;
-  let XX := fresh "X" in
-  let xx := fresh "x" in
-  let A1 := fresh A in
-  let A2 := fresh A in
-  let ll := fresh "l" in
-  let lll := fresh "l" in
-  let tt := fresh "t" in
-  let IHll := fresh "IHl" in
-  induction A as [ XX ll | A1 ? A2 ? | xx A | xx A ]; simpl; intros;
-  [ rewrite ? flat_map_concat_map;
-    try f_equal; try (induction ll as [ | tt lll IHll ]; simpl; intuition;
-                      rewrite IHll; f_equal; intuition)
-  | try (f_equal; intuition)
-  | try (repeat case_analysis; intuition; f_equal; intuition; (rnow idtac); fail)
-  | try (repeat case_analysis; intuition; f_equal; intuition; (rnow idtac); fail) ];
-  try (now (rnow idtac)); try (now rcauto).
+Hint Rewrite (@fsize_dbsubs vatom tatom fatom Ncon Bcon Qcon) : term_db.
+Hint Rewrite (@fsize_subs vatom tatom fatom Ncon Bcon Qcon nat) : term_db.
+Hint Rewrite (@tvars_tdbsubs_fclosed vatom tatom) using intuition; fail : term_db.
+Hint Rewrite (@freevars_dbsubs_fclosed vatom tatom fatom Ncon Bcon Qcon nat)
+                 using intuition; fail : term_db.
+Hint Rewrite (@subs_dbsubs vatom tatom fatom Ncon Bcon Qcon nat)
+                         using try (intuition; fail);
+                              (try apply fclosed_notvars); intuition; fail : term_db.
+Hint Rewrite <- (@lift_dbsubs vatom tatom fatom Ncon Bcon Qcon) : term_db.
+Hint Rewrite (@dbsubs_z_fup vatom tatom fatom Ncon Bcon Qcon) : term_db.
 
-(** lift indexes above [k] in [formula] [A] *)
-Fixpoint fup k A :=
-match A with
-| var X l => var X (map (tup k) l)
-| imp B C => imp (fup k B) (fup k C)
-| frl x B => frl x (fup k B)
-| exs x B => exs x (fup k B)
-end.
-Notation fupz := (fup 0).
-
-Lemma fup_fup_com : forall k A, fup (S k) (fup 0 A) = fup 0 (fup k A).
-Proof. formula_induction A. Qed.
-Hint Rewrite fup_fup_com : term_db.
-
-
-(** substitutes [term] [u] for variable [x] in [formula] [A] *)
-(* capture is not avoided *)
-Fixpoint subs x u A :=
-match A with
-| var X l => var X (map (tsubs x u) l)
-| imp B C => imp (subs x u B) (subs x u C)
-| frl y B => frl y (if (eqb y x) then B else subs x u B)
-| exs y B => exs y (if (eqb y x) then B else subs x u B)
-end.
-
-Lemma fup_subs_com : forall k x u A,
-  fup k (subs x u A) = subs x (tup k u) (fup k A).
-Proof. formula_induction A. Qed.
-Hint Rewrite fup_subs_com : term_db.
-
-(** substitutes [term] [u] for index [n] in [formula] [A] *)
-(* capture is not avoided *)
-Fixpoint nsubs n u A :=
-match A with
-| var X l => var X (map (ntsubs n u) l)
-| imp B C => imp (nsubs n u B) (nsubs n u C)
-| frl x B => frl x (nsubs n u B)
-| exs x B => exs x (nsubs n u B)
-end.
-
-Lemma nsubs_fup_com : forall k u A,
-  nsubs (S k) (tup 0 u) (fup 0 A) = fup 0 (nsubs k u A).
-Proof. formula_induction A. Qed.
-Hint Rewrite nsubs_fup_com : term_db.
-
-Lemma nsubs_z_fup : forall u A, nsubs 0 u (fup 0 A) = A.
-Proof. formula_induction A. Qed.
-Hint Rewrite nsubs_z_fup : term_db.
-
-Lemma nsubs_subs_com : forall x v n u, ~ In x (freevars u) -> forall A,
-  nsubs n u (subs x v A) = subs x (ntsubs n u v) (nsubs n u A).
-Proof. formula_induction A. Qed.
-Hint Rewrite nsubs_subs_com using try (intuition ; fail) ;
-                                  (try apply closed_nofreevars) ; intuition ; fail : term_db.
-
-
-(** size of formulas *)
-Fixpoint fsize A :=
-match A with
-| var _ _ => 1
-| imp B C => S (fsize B + fsize C)
-| frl _ B | exs _ B => S (fsize B)
-end.
-
-Lemma fsize_fup : forall k A, fsize (fup k A) = fsize A.
-Proof. formula_induction A. Qed.
-Hint Rewrite fsize_fup : term_db.
-
-Lemma fsize_subs : forall u x A, fsize (subs x u A) = fsize A.
-Proof. formula_induction A. Qed.
-Hint Rewrite fsize_subs : term_db.
-
-Lemma fsize_nsubs : forall u n A, fsize (nsubs n u A) = fsize A.
-Proof. formula_induction A. Qed.
-Hint Rewrite fsize_nsubs : term_db.
+Hint Resolve (@fclosed_fdblift vatom tatom) : term_db.
+Hint Resolve (@fclosed_fdbsubs vatom tatom) : term_db.
 
 
 (** * Proofs *)
@@ -156,11 +57,11 @@ Inductive prove : list formula -> formula -> Type :=
 | ax : forall l1 l2 A, prove (l1 ++ A :: l2) A
 | impi { l A B } : prove (A :: l) B -> prove l (imp A B)
 | impe { l B } : forall A, prove l (imp A B) -> prove l A -> prove l B
-| frli { x l A } : prove (map fupz l) (subs x (dvar 0) (fupz A)) -> prove l (frl x A)
+| frli { x l A } : prove (map (fun F => F↑) l) A↑[dvar 0//x] -> prove l (frl x A)
 | frle { x l A } : forall u, closed u -> prove l (frl x A) -> prove l (subs x u A)
 | exsi { x l A } : forall u, closed u -> prove l (subs x u A) -> prove l (exs x A)
 | exse { l C } : forall x A, prove l (exs x A) ->
-                             prove (subs x (dvar 0) (fupz A) :: map fupz l) (fupz C) -> prove l C.
+                             prove (A↑[dvar 0//x] :: map (fun F => F↑) l) C↑ -> prove l C.
 Hint Constructors prove : term_db.
 Global Arguments impe { l B } _ _ _.
 Global Arguments exse { l C } _ _ _.
@@ -176,10 +77,11 @@ Inductive nprove : list formula -> formula -> Type := (* neutral terms *)
 with rprove : list formula -> formula -> Type := (* normal forms *)
 | rninj { l A } : nprove l A -> rprove l A
 | rimpi { l A B } : rprove (A :: l) B -> rprove l (imp A B)
-| rfrli { x l A } : rprove (map fupz l) (subs x (dvar 0) (fupz A)) -> rprove l (frl x A)
+| rfrli { x l A } : rprove (map (dbsubs ⇑) l) A↑[dvar 0//x] -> rprove l (frl x A)
 | rexsi { x l A } : forall u, closed u -> rprove l (subs x u A) -> rprove l (exs x A)
-| rexse { l C } : forall x A, nprove l (exs x A) ->
-                              rprove (subs x (dvar 0) (fupz A) :: map fupz l) (fupz C) -> rprove l C.
+| rexse { l C } : forall x A,
+                     nprove l (exs x A) ->
+                     rprove (A↑[dvar 0//x] :: map (dbsubs ⇑) l) C↑ -> rprove l C.
 Hint Constructors nprove rprove : term_db.
 Global Arguments nimpe { l B } _ _ _.
 Global Arguments rexse { l C } _ _ _ _.
@@ -219,74 +121,49 @@ match pi with
 end.
 
 
-(** substitutes [term] [u] for index [n] in normal form and decreases indexes above [n] *)
-Theorem rnpsubs n u (Hc : closed u) {l A} :
-   (nprove l A -> nprove (map (nsubs n u) l) (nsubs n u A))
- * (rprove l A -> rprove (map (nsubs n u) l) (nsubs n u A)).
+(** apply [r] in normal form *)
+Theorem rnpdbsubs r (Hc : fclosed r) {l A} :
+   (nprove l A -> nprove (map (dbsubs r) l) A⟦r⟧)
+ * (rprove l A -> rprove (map (dbsubs r) l) A⟦r⟧).
 Proof with try eassumption.
 revert l A.
-enough ((forall l A, nprove l A -> forall n u, closed u -> nprove (map (nsubs n u) l) (nsubs n u A))
-      * (forall l A, rprove l A -> forall n u, closed u -> rprove (map (nsubs n u) l) (nsubs n u A)))
-  as He by (split ; intros ; apply He ; assumption).
-clear n u Hc ; apply rnprove_mutrect ; intros ; (try simpl in X) ;
-  (try assert (IH1 := X n0 u H)) ; (try assert (IH2 := X0 n0 u H)) ; 
-  (try (econstructor ; (eassumption + intuition) ; fail)).
-- rewrite map_app ; apply nax.
+enough ((forall l A, nprove l A ->
+                       forall r, fclosed r -> nprove (map (dbsubs r) l) A⟦r⟧)
+      * (forall l A, rprove l A ->
+                       forall r, fclosed r -> rprove (map (dbsubs r) l) A⟦r⟧))
+  as He by (split; intros; apply He; assumption).
+clear r Hc; apply rnprove_mutrect; intros; (try simpl in X);
+  (try assert (IH1 := X r H)); (try assert (IH2 := X0 r H));
+  (try (econstructor; (eassumption + intuition); fail)).
+- rewrite map_app; apply nax.
 - rnow idtac then rnow eapply nfrle.
-- assert (closed (tup 0 u)) by rnow idtac.
-  specialize X with (S n) (tup 0 u).
-  rewrite map_map, (map_ext _ _ (nsubs_fup_com _ _)), <- map_map in X.
-  rnow autorewrite with term_db in X.
-- rnow specialize X with n u0 then rnow eapply (rexsi (ntsubs n u0 u)).
-- rewrite <- (freevars_tup 0) in H.
-  clear IH2 ; assert (IH2 := X0 (S n0) (tup 0 u) H) ; simpl in IH2.
-  rewrite map_map in IH2 ; rewrite (map_ext _ _ (nsubs_fup_com _ _)) in IH2 ;
-    rewrite <- map_map in IH2.
+- assert (fclosed (↑r0)) by rnow idtac.
+  specialize X with (↑r0).
+  revert X; rnow idtac.
+  rewrite map_map, <- (map_ext _ _ (lift_dbsubs _)), <- map_map in X0; intuition.
+- rnow specialize X with r0 then rnow eapply (rexsi (tdbsubs r0 u)).
+- assert (fclosed (↑r0)) as Hup by rnow idtac.
+  assert (IH := X0 (↑r0) Hup); simpl in IH.
+  rewrite map_map, <- (map_ext _ _ (lift_dbsubs _)), <- map_map in IH.
   rnow eapply rexse.
 Qed.
 
 Lemma rpsubsz_r {l A x u} : closed u ->
-  rprove (map fupz l) (subs x (dvar 0) (fupz A)) -> rprove l (subs x u A).
+  rprove (map (dbsubs ⇑) l) A↑[dvar 0//x] -> rprove l (subs x u A).
 Proof.
 intros Hc pi.
-apply (rnpsubs 0 u) in pi; [ | assumption ].
-rnow simpl in pi then simpl in pi.
-now rewrite map_map, (map_ext _ _ (nsubs_z_fup _)), map_id in pi.
+apply (rnpdbsubs (u//↓0)) in pi; [ | intuition ].
+rnow simpl in pi then cbn in pi.
+now rewrite map_map, (map_ext _ _ (dbsubs_z_fup _)), map_id in pi.
 Qed.
 
 Lemma rpsubsz_l {l A x u C} : closed u ->
-  rprove (subs x (dvar 0) (fupz A) :: map fupz l) (fupz C) -> rprove (subs x u A :: l) C.
+  rprove (A↑[dvar 0//x] :: map (dbsubs ⇑) l) C↑ -> rprove (subs x u A :: l) C.
 Proof.
 intros Hc pi.
-apply (rnpsubs 0 u) in pi; [ | assumption ].
+apply (rnpdbsubs (u//↓0)) in pi; [ | intuition ].
 rnow simpl in pi then simpl in pi.
-now rewrite map_map, (map_ext _ _ (nsubs_z_fup _)), map_id in pi.
-Qed.
-
-
-(** lift indexes above [k] in normal form *)
-Theorem rnpup k {l A} :
-   (nprove l A -> nprove (map (fup k) l) (fup k A))
- * (rprove l A -> rprove (map (fup k) l) (fup k A)).
-Proof.
-revert l A.
-enough ((forall l A, nprove l A -> forall k, nprove (map (fup k) l) (fup k A))
-      * (forall l A, rprove l A -> forall k, rprove (map (fup k) l) (fup k A)))
-  as He by (split ; intros ; apply He ; assumption).
-clear k ; apply rnprove_mutrect ; intros;
-  (try assert (IH1 := X k)) ; (try assert (IH2 := X0 k)) ;
-  (try (econstructor ; eassumption ; fail)).
-- rewrite map_app ; apply nax.
-- rnow idtac then rnow apply nfrle.
-- clear IH1 ; assert (IH := X (S k)).
-  rnow change (dvar 0) with (tup (S k) (dvar 0)) in X.
-  rewrite map_map, (map_ext _ _ (fup_fup_com _)), <- map_map in IH.
-  now apply rfrli.
-- rnow idtac then rnow apply (rexsi (tup k u)).
-- clear IH2 ; assert (IH2 := X0 (S k)) ; simpl in IH2.
-  rnow change (dvar 0) with (tup (S k) (dvar 0)) in X.
-  rewrite map_map, (map_ext _ _ (fup_fup_com _)), <- map_map in IH2.
-  rnow apply (rexse x (fup k A)).
+now rewrite map_map, (map_ext _ _ (dbsubs_z_fup _)), map_id in pi.
 Qed.
 
 
@@ -320,28 +197,28 @@ Qed.
 Lemma imp_reduction : forall A B l, rprove l (imp A B) ->
 (forall D l B, fsize D = fsize A -> rprove (D :: l) B -> rprove l D -> rprove l B) -> 
   rprove l A -> rprove l B.
-Proof with try eassumption ; try reflexivity.
+Proof.
 intros A B l pi.
 remember (imp A B) as C ; revert A B HeqC ; induction pi ;
   intros A1 B1 HeqC ; inversion HeqC ; subst ; intros Hsub pi2.
-- apply rninj ; eapply nimpe...
-- eapply Hsub...
-- eapply rexse...
-  eapply (IHpi (fupz A1) (fupz B1))...
+- apply rninj; eapply nimpe; eassumption.
+- now eapply Hsub.
+- eapply rexse; [ eassumption | ].
+  eapply (IHpi (A1↑) (B1↑)); [ reflexivity | | ].
   + clear - Hsub ; intros D l B Hs pi1 pi2.
-    rnow eapply (Hsub D)...
-  + rewrite <- (app_nil_l (map fupz l)) ; rewrite app_comm_cons ; rewrite <- (app_nil_l _).
-    eapply weakening...
-    apply rnpup...
+    rnow eapply (Hsub D).
+  + rewrite <- (app_nil_l (map (dbsubs ⇑) l)) ; rewrite app_comm_cons ; rewrite <- (app_nil_l _).
+    eapply weakening; [ | reflexivity ].
+    now apply rnpdbsubs.
 Qed.
 
 Lemma frl_reduction : forall A x l, rprove l (frl x A) ->
   forall u, closed u -> rprove l (subs x u A).
 Proof with try eassumption ; try reflexivity.
 intros A x l pi.
-remember (frl x A) as C ; revert A x HeqC ; induction pi ;
-  intros A1 x1 HeqC ; inversion HeqC ; subst ; intros u Hc.
-- apply rninj ; eapply nfrle...
+remember (frl x A) as C; revert A x HeqC; induction pi;
+  intros A1 x1 HeqC; inversion HeqC; subst; intros u Hc.
+- apply rninj; eapply nfrle...
 - eapply rpsubsz_r in pi...
 - eapply rexse...
   rnow simpl in IHpi then rnow (eapply IHpi).
@@ -349,26 +226,25 @@ Qed.
 
 Lemma exs_reduction : forall A x l, rprove l (exs x A) ->
 (forall D l B, fsize D = fsize A -> rprove (D :: l) B -> rprove l D -> rprove l B) -> 
-  forall C, rprove (subs x (dvar 0) (fupz A) :: map fupz l) (fupz C) -> rprove l C.
-Proof with try eassumption ; try reflexivity.
+  forall C, rprove (A↑[dvar 0//x] :: map (dbsubs ⇑) l) C↑ -> rprove l C.
+Proof.
 intros A x l pi.
-remember (exs x A) as A' ; revert A x HeqA' ; induction pi ;
-  intros A' x1 HeqA' ; inversion HeqA' ; subst ; intros Hsub C pi2.
-- eapply rexse...
-- eapply rpsubsz_l in pi2...
-  rnow apply (Hsub (subs x1 u A')).
+remember (exs x A) as A'; revert A x HeqA'; induction pi;
+  intros A' x1 HeqA'; inversion HeqA'; subst; intros Hsub C pi2.
+- eapply rexse; eassumption.
+- eapply rpsubsz_l in pi2; [ | eassumption ].
+  rnow apply (Hsub (A'[u//x1])).
 - rnow simpl in IHpi.
-  eapply rexse...
+  eapply rexse; [ eassumption | ].
   eapply IHpi ; [ reflexivity | | ].
   + clear - Hsub ; intros D l B Hs pi1 pi2.
-    rnow eapply (Hsub D)...
-  + simpl ; rewrite <- (app_nil_l (subs x _ _ :: _)) ; rewrite app_comm_cons ;
-      rewrite <- (app_nil_l (map fupz _)) ; rewrite app_comm_cons.
-    eapply weakening...
-    apply (rnpup 1) in pi2.
+    rnow eapply (Hsub D).
+  + simpl ; rewrite <- (app_nil_l (subs x _ _ :: _)) ; rewrite app_comm_cons;
+      rewrite <- (app_nil_l (map (dbsubs ⇑) _)) ; rewrite app_comm_cons.
+    eapply weakening; [ | reflexivity ].
+    apply (rnpdbsubs (↑⇑)) in pi2; intuition.
     rnow simpl in pi2 then simpl in pi2.
-    rewrite map_map in pi2 ; rewrite (map_ext _ _ (fup_fup_com _)) in pi2 ;
-      rewrite <- map_map in pi2...
+    now rewrite map_map, <- (map_ext _ _ (lift_dbsubs _)), <- map_map in pi2.
 Qed.
 
 Lemma substitution : forall n m A, fsize A = n ->
@@ -437,18 +313,18 @@ apply (lt_wf_double_rect (fun n m =>
     rewrite <- (app_nil_l _).
   eapply weakening...
 - apply rfrli ; rewrite map_app.
-  apply (rnpup 0) in pi1.
+  apply (rnpdbsubs ⇑) in pi1; intuition.
   revert pi1 pi2 Hpi ; rewrite ? map_app ; simpl ; intros pi1 pi2 Hpi.
   rnow refine (snd (IHm _ _ _ _) _ _ _ pi2 _ _)...
 - eapply rexsi...
   refine (snd (IHm _ _ _ _) _ _ _ pi2 _ _)...
 - rewrite <- (app_nil_l _) in pi1.
-  assert (pi1' := snd weakening _ _ (snd (rnpup 0) pi1)
-                  (subs x (dvar 0) (fupz A0) :: nil) nil _ eq_refl) ; simpl in pi1'.
+  assert (pi1' := snd weakening _ _ (snd (rnpdbsubs ⇑ fclosed_fup) pi1)
+                  (A0↑[dvar 0//x] :: nil) nil _ eq_refl) ; simpl in pi1'.
   rewrite map_app in pi1' ; rewrite app_comm_cons in pi1'.
   revert pi2 pi1' Hpi ; rewrite ? map_app ; simpl ; rewrite app_comm_cons ;
     intros pi2 pi1' Hpi.
-  assert (fsize (fupz A) = fsize A) as Hup by (rnow idtac).
+  assert (fsize (A↑) = fsize A) as Hup by (rnow idtac).
   eapply (snd (IHm _ Hpi _ Hup) _ _ _ pi2) in pi1'...
   destruct (Compare_dec.le_lt_dec (fsize (exs x A0)) (fsize A)).
   + eapply (snd (fst (IHm _ Hpi _ eq_refl)) _ _ _ n) in pi1...
@@ -481,331 +357,6 @@ intros l A pi ; induction pi ;
 Qed.
 
 
-(** * Free variables in [formula] *)
-Fixpoint ffreevars A :=
-match A with
-| var _ l => flat_map freevars l
-| imp B C => ffreevars B ++ ffreevars C
-| frl x B | exs x B => remove eq_dt_dec x (ffreevars B)
-end.
-
-Lemma in_ffreevars_frl : forall x y, y <> x -> forall A,
-  In x (ffreevars A) -> In x (ffreevars (frl y A)).
-Proof. formula_induction A; apply notin_remove; intuition; now rewrite <- flat_map_concat_map. Qed.
-
-Lemma ffreevars_fup : forall k A, ffreevars (fup k A) = ffreevars A.
-Proof. formula_induction A. Qed.
-Hint Rewrite ffreevars_fup : term_db.
-
-Lemma nfree_subs : forall x u A, ~ In x (ffreevars A) -> subs x u A = A.
-Proof. formula_induction A; try rcauto.
-- rnow apply nfree_tsubs then apply H.
-- rnow apply H.
-- rnow rewrite IHA.
-  now apply H; apply in_ffreevars_frl.
-- rnow rewrite IHA.
-  now apply H; apply in_ffreevars_frl.
-Qed.
-Hint Rewrite nfree_subs using intuition ; fail : term_db.
-
-Lemma ffreevars_subs_closed : forall x u, closed u -> forall A,
-  ffreevars (subs x u A) = remove eq_dt_dec x (ffreevars A).
-Proof. formula_induction A ; rewrite ? remove_app; try now f_equal.
-- now f_equal; apply freevars_tsubs_closed.
-- case_analysis.
-  + symmetry; apply remove_remove_eq.
-  + now rewrite remove_remove_neq by (now intros Heq'; apply Heq); f_equal.
-- case_analysis.
-  + symmetry; apply remove_remove_eq.
-  + now rewrite remove_remove_neq by (now intros Heq'; apply Heq); f_equal.
-Qed.
-Hint Rewrite ffreevars_subs_closed using intuition; fail : term_db.
-
-Lemma ffreevars_subs : forall x y u A, In x (ffreevars (subs y u A)) ->
-  (In x (freevars u) /\ In y (ffreevars A)) \/ (In x (ffreevars A) /\ x <> y).
-Proof. formula_induction A; try in_solve.
-- revert H; induction l; simpl; intros Hin.
-  + inversion Hin.
-  + apply in_app_or in Hin; destruct Hin as [Hin|Hin].
-    * apply freevars_tsubs in Hin; in_solve.
-    * apply IHl in Hin; in_solve.
-- refine ?[mygoal]. Existential 1 := ?mygoal.
-  revert H; case_analysis; intros H.
-  + right; intuition.
-    apply in_remove in H; intuition.
-  + assert (Hin := proj1 (in_remove _ _ _ _ H)).
-    apply IHA in Hin; destruct Hin as [Hin|Hin]; [left|right]; intuition;
-      apply notin_remove; intuition.
-    subst; revert H; apply remove_In.
-Qed.
-
-Lemma subs_subs_eq : forall x u v A, subs x u (subs x v A) = subs x (tsubs x u v) A.
-Proof. formula_induction A. Qed.
-Hint Rewrite subs_subs_eq : term_db.
-
-Lemma subs_subs_com_closed : forall x v y u, x <> y -> closed u -> closed v ->
-  forall A, subs y u (subs x v A) = subs x (tsubs y u v) (subs y u A).
-Proof. formula_induction A. Qed.
-Hint Rewrite subs_subs_com_closed using intuition; fail : term_db.
-
-Fixpoint good_for x y A :=
-match A with
-| var X l => True
-| imp B C => good_for x y B /\ good_for x y C
-| frl z B | exs z B => In x (ffreevars (exs z B)) -> good_for x y B /\ y <> z
-end.
-
-Lemma good_for_subs : forall x y z t A, closed t -> x <> z ->
-  good_for x y A -> good_for x y (subs z t A).
-Proof. intros x y z t A; revert t; formula_induction A.
-- refine ?[mygoal]. Existential 1 := ?mygoal.
-  assert (incl (remove eq_dt_dec x0 (ffreevars (subs z t A))) (remove eq_dt_dec x0 (ffreevars A)))
-    as Hincl.
-  { apply remove_incl.
-    intros a Ha.
-    apply ffreevars_subs in Ha; destruct Ha as [Ha|Ha]; intuition.
-    exfalso; now rewrite H in H3. }
-  revert H1 H2; repeat case_analysis; intros H1 H2; intuition.
-  + apply IHA; intuition.
-    apply H1; intuition.
-  + apply H1; intuition.
-Qed.
-
-Lemma subs_subs_com_good : forall x v y u, x <> y -> closed u -> forall A,
-  Forall (fun y => good_for x y A) (freevars v) ->
-  subs y u (subs x v A) = subs x (tsubs y u v) (subs y u A).
-Proof. induction A; simpl; intros Hb; f_equal.
-- rnow rewrite 2 map_map; apply map_ext; rcauto.
-- apply IHA1; eapply Forall_impl; [ | eassumption ]; simpl; intuition.
-- apply IHA2; eapply Forall_impl; [ | eassumption ]; simpl; intuition.
-- refine ?[mygoal]. Existential 1 := ?mygoal.
-  repeat case_analysis; intuition.
-  + destruct (in_dec eq_dt_dec y (freevars v));
-     [ destruct (in_dec eq_dt_dec x (ffreevars A)) | ]; rcauto.
-    exfalso.
-    specialize_Forall Hb with y; apply Hb; intuition.
-    now apply notin_remove.
-  + destruct (in_dec eq_dt_dec x (ffreevars A)).
-    * apply IHA.
-      apply Forall_forall; intros z Hinz.
-      specialize_Forall Hb with z; apply Hb.
-      apply notin_remove; intuition.
-    * rewrite 2 (nfree_subs x); [ reflexivity | | assumption ].
-      intros Hin; apply n.
-      rewrite ffreevars_subs_closed in Hin; [ | assumption ].
-      now apply in_remove in Hin.
-Qed.
-Hint Rewrite subs_subs_com_good using intuition; fail : term_db.
-
-Lemma ffreevars_to_subs : forall A x y t, good_for y x A ->
-  In y (ffreevars A) -> In x (freevars t) -> In x (ffreevars (subs y t A)).
-Proof. formula_induction A; try in_solve.
-- revert H0 H1; clear; induction l; intros Hin1 Hin2; simpl; intuition.
-  simpl in Hin1.
-  apply in_or_app; apply in_app_or in Hin1; destruct Hin1 as [Hin1|Hin1]; [left|right]; rcauto.
-  now apply freevars_to_tsubs.
-- refine ?[mygoal]. Existential 1 := ?mygoal.
-  apply in_remove in H0; destruct H0 as [Hin Hneq].
-  case_analysis; intuition.
-  assert (Hin2 := notin_remove eq_dt_dec _ _ x Hneq Hin).
-  apply notin_remove; intuition.
-Qed.
-
-(* ** Iterated substitution *)
-
-Fixpoint remove_snd {T} x (L : list (vatom * T)) :=
-match L with
-| nil => nil
-| (y, F) :: TL => if eqb x y then remove_snd x TL else (y, F) :: remove_snd x TL
-end.
-
-Lemma remove_snd_remove {T} x (L : list (vatom * T)) :
-  remove eq_dt_dec x (map fst L) = map fst (remove_snd x L).
-Proof.
-induction L; simpl; [ reflexivity | rewrite IHL ]; destruct a; simpl.
-repeat case_analysis; intuition.
-Qed.
-Hint Rewrite (@remove_snd_remove formula) : term_db.
-
-Lemma remove_snd_notin {T} x (L : list (vatom * T)) :
-  forall y a, x <> y -> In (y, a) L -> In (y, a) (remove_snd x L).
-Proof.
-induction L; simpl; intros y b Hneq Hin; [ assumption | destruct a ].
-destruct Hin as [Hin|Hin]; case_analysis; intuition.
-exfalso; apply Hneq.
-now inversion Hin.
-Qed.
-
-Lemma snd_remove_snd {T} x (L : list (vatom * T)) :
-  incl (map snd (remove_snd x L)) (map snd L).
-Proof.
-induction L; simpl; intros z Hz; intuition.
-destruct a; simpl.
-revert Hz; case_analysis; intros Hz; intuition.
-Qed.
-
-Lemma NoDup_remove_snd {T} x (L : list (vatom * T)) :
-  NoDup (map snd L) -> NoDup (map snd (remove_snd x L)).
-Proof.
-induction L; simpl; intros Hnd; [ constructor | destruct a ].
-inversion_clear Hnd.
-case_analysis; intuition.
-constructor; intuition.
-apply snd_remove_snd in H2.
-now apply H.
-Qed.
-
-(* iterated substitution *)
-Definition multi_subs L A := fold_left (fun F '(x,u) => subs x u F) L A.
-
-Lemma multi_subs_nil : multi_subs nil = id.
-Proof. reflexivity. Qed.
-Hint Rewrite multi_subs_nil : term_db.
-
-Lemma multi_subs_var : forall L X l, multi_subs L (var X l) = var X (map (multi_tsubs L) l).
-Proof.
-induction L; intros X l; simpl.
-- now rewrite multi_tsubs_nil, map_id.
-- now destruct a; rewrite IHL, map_map.
-Qed.
-Hint Rewrite multi_subs_var : term_db.
-
-Lemma multi_subs_imp : forall L A B, multi_subs L (imp A B) = imp (multi_subs L A) (multi_subs L B).
-Proof. now induction L; intros A B; simpl; [ | destruct a; rewrite IHL ]. Qed.
-Hint Rewrite multi_subs_imp : term_db.
-
-Lemma multi_subs_frl : forall L x A, multi_subs L (frl x A) = frl x (multi_subs (remove_snd x L) A).
-Proof.
-induction L; intros x A; simpl; [ reflexivity | destruct a; simpl ].
-case_analysis; rewrite IHL; f_equal.
-Qed.
-Hint Rewrite multi_subs_frl : term_db.
-
-Lemma multi_subs_exs : forall L x A, multi_subs L (exs x A) = exs x (multi_subs (remove_snd x L) A).
-Proof.
-induction L; intros x A; simpl; [ reflexivity | destruct a; simpl ].
-case_analysis; rewrite IHL; f_equal.
-Qed.
-Hint Rewrite multi_subs_exs : term_db.
-
-Lemma multi_subs_closed : forall L A, ffreevars A = nil -> multi_subs L A = A.
-Proof.
-induction L; intros A Hc; [ reflexivity | destruct a; simpl ].
-(rnow rewrite nfree_subs); rewrite Hc in H; inversion H.
-Qed.
-Hint Rewrite multi_subs_closed using intuition; fail : term_db.
-
-Lemma multi_subs_is_closed : forall L A,
-  Forall (fun z => closed z) (map snd L) -> incl (ffreevars A) (map fst L) ->
-  ffreevars (multi_subs L A) = nil.
-Proof.
-induction L; simpl; intros A Hc Hf.
-- now apply incl_nil_inv in Hf; subst.
-- destruct a; simpl; simpl in Hc, Hf; inversion_clear Hc as [ | ? ? Hc2 HcF].
-  apply IHL; intuition.
-  intros z Hinz.
-  rewrite ffreevars_subs_closed in Hinz by assumption.
-  apply in_remove in Hinz; destruct Hinz as [Hinz Hneq].
-  apply Hf in Hinz; inversion Hinz; [ exfalso | ]; intuition.
-Qed.
-
-Lemma multi_subs_ffreevars : forall L x A, 
-  Forall (fun z => closed z) (map snd L) ->
-  In x (ffreevars (multi_subs L A)) -> In x (ffreevars A).
-Proof.
-induction L; intros x A Hc Hin; [ assumption | destruct a; simpl in Hc, Hin ].
-inversion_clear Hc as [ | ? ? Hct HcF ].
-apply IHL in Hin; trivial.
-apply ffreevars_subs in Hin; destruct Hin as [[Hin _]| ]; intuition.
-exfalso; rewrite Hct in Hin; inversion Hin.
-Qed.
-
-Lemma multi_subs_subs : forall L x v,
-  Forall (fun z => closed z) (map snd L) ->
-  forall A, Forall (fun y => good_for x y A) (freevars v) ->
-  multi_subs L (subs x v A) = subs x (multi_tsubs L v) (multi_subs (remove_snd x L) A).
-Proof.
-induction L; simpl; intros x v Hc A Hb; [ reflexivity | destruct a; simpl; simpl in Hc ].
-inversion_clear Hc as [ | ? ? Hct HcF ].
-case_analysis; rewrite <- IHL; intuition; f_equal; rcauto.
-- apply Forall_incl with (freevars v); intuition.
-  apply incl_remove.
-- apply Forall_incl with (freevars v).
-  + apply incl_remove.
-  + apply Forall_impl with (fun y => good_for x y A); trivial.
-    intros a; now apply good_for_subs.
-Qed.
-Hint Rewrite multi_subs_subs using intuition; fail : term_db.
-
-Lemma multi_subs_remove : forall L A x,
-  Forall (fun z => closed z) (map snd L) ->
-  ~ In x (ffreevars A) -> multi_subs (remove_snd x L) A = multi_subs L A.
-Proof.
-induction L; simpl; intros A x Hc Hin; [ reflexivity | destruct a; simpl; simpl in Hc ].
-inversion_clear Hc as [ | ? ? Hct HcF ].
-case_analysis; rcauto.
-apply IHL; try assumption.
-intros Hin2; apply Hin.
-apply ffreevars_subs in Hin2.
-destruct Hin2 as [[Hin2 _]|[Hin2 _]]; trivial.
-exfalso; rewrite Hct in Hin2; inversion Hin2.
-Qed.
-Hint Rewrite multi_subs_remove using intuition; fail : term_db.
-
-Lemma fup_multi_subs : forall L k A,
-  fup k (multi_subs L A) = multi_subs (map (fun x => (fst x, tup k (snd x))) L) (fup k A).
-Proof. induction L; simpl; intros k A; [ | rewrite IHL ]; rcauto. Qed.
-Hint Rewrite fup_multi_subs : term_db.
-
-Lemma multi_subs_ext : forall L A,
-  Forall (fun z => closed z) (map snd L) -> incl (ffreevars A) (map fst L) ->
-  forall L', multi_subs L A = multi_subs (L ++ L') A.
-Proof.
-intros L A Hcl Hsub L'.
-unfold multi_subs at 2; rewrite fold_left_app.
-rewrite multi_subs_closed
-  with (A:= fold_left (fun F '(x,u) => subs x u F) L A); trivial.
-now apply multi_subs_is_closed.
-Qed.
-
-(* All variables occurring (free or bound or for quantification) in a formula *)
-Fixpoint allvars A :=
-match A with
-| var _ l => flat_map freevars l
-| imp B C => allvars B ++ allvars C
-| frl x B | exs x B => x :: allvars B
-end.
-
-Lemma ffreevars_allvars : forall A, incl (ffreevars A) (allvars A).
-Proof. formula_induction A.
-- refine ?[mygoal]. Existential 1 := ?mygoal.
-  eapply incl_tran; [ apply incl_remove | ].
-  eapply incl_tran; [ apply IHA | intuition ].
-Qed.
-
-Lemma bisubs : forall x y A, ~ In x (allvars A) ->
-  subs x (tvar y) (subs y (tvar x) A) = A.
-Proof. formula_induction A; f_equal.
-- apply tbisubs.
-  intros Hin; apply H; simpl; intuition.
-- apply H; simpl; intuition.
-- refine ?[mygoal]. Existential 1 := ?mygoal.
-  repeat case_analysis; intuition.
-  apply nfree_subs.
-  intros Hin; apply H1.
-  now apply ffreevars_allvars.
-Qed.
-
-(* Eigen variables *)
-
-Fixpoint eigen_max A :=
-match A with
-| var _ l => list_max (map teigen_max l)
-| imp B C => max (eigen_max B) (eigen_max C)
-| frl _ B | exs _ B => eigen_max B
-end.
-
-
 (** * Sub-Formula Property *)
 
 (** Sub-formula Relation *)
@@ -814,27 +365,29 @@ Inductive subform : formula -> formula -> Prop :=
 | sub_imp_l : forall A B C, subform A B -> subform A (imp B C)
 | sub_imp_r : forall A B C, subform A B -> subform A (imp C B)
 | sub_frl : forall A x u B, subform A (subs x u B) -> subform A (frl x B)
-| sub_ex : forall A x u B, subform A (subs x u B) -> subform A (exs x B)
-| sub_frl_n : forall A x B, subform A (subs x (dvar 0) (fupz B)) -> subform A (frl x B)
-| sub_ex_n : forall A x B, subform A (subs x (dvar 0) (fupz B)) -> subform A (exs x B)
-| sub_fup : forall A B, subform A (fupz B) -> subform A B.
+| sub_exs : forall A x u B, subform A (subs x u B) -> subform A (exs x B)
+| sub_frl_n : forall A x B, subform A B↑[dvar 0//x] -> subform A (frl x B)
+| sub_ex_n : forall A x B, subform A B↑[dvar 0//x] -> subform A (exs x B)
+| sub_fup : forall A B, subform A B↑ -> subform A B.
 
 Lemma subform_trans : forall A B C, subform A B -> subform B C -> subform A C.
 Proof.
 now intros A B C Hl Hr; revert A Hl; induction Hr; intros A' Hl; try (econstructor; apply IHHr).
 Qed.
 
-Lemma subform_fupz : forall A B, subform A B -> subform (fupz A) (fupz B).
+Lemma subform_fupz : forall A B, subform A B -> subform A↑ B↑.
 Proof.
 intros A B Hs; induction Hs; try (now econstructor; eauto).
-- rewrite fup_subs_com in IHHs; now econstructor; eauto.
-- rewrite fup_subs_com in IHHs; now econstructor; eauto.
+- rcauto; econstructor; eauto.
+- rcauto; econstructor; eauto.
 - eapply subform_trans; [ apply IHHs | ].
-  simpl; rewrite fup_subs_com; do 2 econstructor.
-  rewrite fup_subs_com; apply sub_id.
+  apply sub_fup; simpl.
+  apply (sub_frl _ (dvar 1)).
+  rcauto; apply sub_id.
 - eapply subform_trans; [ apply IHHs | ].
-  simpl; rewrite fup_subs_com; do 2 econstructor.
-  rewrite fup_subs_com; apply sub_id.
+  apply sub_fup; simpl.
+  apply (sub_exs _ (dvar 1)).
+  rcauto; apply sub_id.
 Qed.
 
 (* restricted notion of sub-formula *)
@@ -842,7 +395,7 @@ Inductive lsubform : formula -> formula -> Prop :=
 | lsub_id : forall A, lsubform A A
 | lsub_imp_r : forall A B C, lsubform (imp A B) C -> lsubform B C
 | lsub_frl : forall A x u B, lsubform (frl x A) B -> lsubform (subs x u A) B
-| lsub_ex : forall A x u B, lsubform (exs x A) B -> lsubform (subs x u A) B.
+| lsub_exs : forall A x u B, lsubform (exs x A) B -> lsubform (subs x u A) B.
 
 Lemma lsubform_trans : forall A B C, lsubform A B -> lsubform B C -> lsubform A C.
 Proof.
@@ -884,7 +437,7 @@ Lemma rnprove_stronger : forall (P Q : formula -> Prop), (forall x, P x -> Q x) 
 Proof. intros; apply rnprove_mutrect ; simpl ; intuition; eapply Forall_impl ; eassumption. Qed.
 
 Proposition prove_with_prop_has_prop : forall (P : formula -> Prop),
- (forall A, P (fupz A) -> P A) ->
+ (forall A, P A↑ -> P A) ->
    (forall l A (pi : nprove l A), nprove_with_prop P pi -> Forall P (A :: l))
  * (forall l A (pi : rprove l A), rprove_with_prop P pi -> Forall P (A :: l)).
 Proof.
@@ -904,8 +457,8 @@ intros P Hfup; apply rnprove_mutrect.
   constructor; intuition.
   inversion_clear H1.
   apply Forall_forall; intros C HC.
-  apply in_map with (f:= fupz) in HC.
-  specialize_Forall H3 with (fupz C); intuition.
+  apply in_map with (f:= dbsubs ⇑) in HC.
+  specialize_Forall H3 with (C↑); intuition.
 - intros x l A u Hc pi1 HP1 pi; inversion_clear pi; intuition.
   constructor; intuition.
   now inversion H1.
@@ -1042,7 +595,8 @@ Theorem subformula_prop :
  * (forall l A (pi : rprove l A), rprove_with_prop (fun B => Exists (subform B) (A :: l)) pi).
 Proof. split; intros l A pi; apply lsubformula_prop. Qed.
 
-Theorem subformula_prop_hered : forall (P : formula -> Prop), (forall A B, subform A B -> P B -> P A) ->
+Theorem subformula_prop_hered : forall (P : formula -> Prop),
+ (forall A B, subform A B -> P B -> P A) ->
    (forall l A (pi : nprove l A), Forall P (A :: l) -> nprove_with_prop P pi)
  * (forall l A (pi : rprove l A), Forall P (A :: l) -> rprove_with_prop P pi).
 Proof.
@@ -1073,27 +627,26 @@ Goal forall A, rprove nil (imp (frl x (frl y A)) (frl y (frl x A))).
 Proof.
 intros; rev_intros; case_analysis.
 - rnow apply nfrle.
-  replace (frl y (fupz (fupz A)))
-     with (subs y (dvar 0) (frl y (fupz (fupz A))))
+  replace (frl y A↑↑)
+     with (subs y (dvar 0) (frl y A↑↑))
     by rcauto.
   rnow apply nfrle then subst; rcauto.
-- rewrite fup_subs_com, subs_subs_com_closed; intuition.
-  rnow apply nfrle.
-  replace (frl y (subs x (dvar 0) (fupz (fupz A))))
-    with (subs x (dvar 0) (frl y (fupz (fupz A))))
+- rewrite subs_dbsubs, subs_subs_closed; intuition.
+  apply nfrle; intuition.
+  replace (frl y A↑↑[dvar 0//x]) with ((frl y A↑↑)[dvar 0//x])
     by (simpl; case_analysis; intuition).
-  rnow apply nfrle.
+  apply nfrle; intuition.
 Qed.
 
 Variable f : tatom.
 Variable P : fatom.
 
-Goal rprove nil (imp (frl x (var P (tconstr f (tvar x :: nil) :: nil)))
-                     (frl x (var P (tconstr f (tconstr f (tvar x :: nil) :: nil) :: nil)))).
+Goal rprove nil (imp (frl x (fvar P (tconstr f (tvar x :: nil) :: nil)))
+                     (frl x (fvar P (tconstr f (tconstr f (tvar x :: nil) :: nil) :: nil)))).
 Proof.
 intros; rev_intros; case_analysis.
-replace (var P (tconstr f (tconstr f (dvar 0 :: nil) :: nil) :: nil))
-   with (subs x (tconstr f (dvar 0 :: nil)) (var P (tconstr f (tvar x :: nil) :: nil)))
+replace (fvar P (tconstr f (tconstr f (dvar 0 :: nil) :: nil) :: nil))
+   with (subs x (tconstr f (dvar 0 :: nil)) (fvar P (tconstr f (tvar x :: nil) :: nil)))
   by (simpl; case_analysis; intuition).
 rnow apply nfrle.
 Qed.
@@ -1108,15 +661,15 @@ Proof. intros A u x Hf; rev_intros; rnow apply (nfrle u). Qed.
 
 Lemma frl_imp : forall A B x, rprove (frl x (imp A B) :: nil) (imp (frl x A) (frl x B)).
 Proof. intros A B x; rev_intros.
-apply (nimpe (subs x (dvar 0) (fupz A))).
-- change (imp (subs x (dvar 0) (fupz A)) (subs x (dvar 0) (fupz B)))
-    with (subs x (dvar 0) (imp (fupz A) (fupz B))).
+apply (nimpe A↑[dvar 0//x]).
+- change (imp A↑[dvar 0//x] B↑[dvar 0//x])
+    with ((imp A↑ B↑)[dvar 0//x]).
   apply nfrle ; [ reflexivity | ] ; simpl.
   auto_nax.
 - now apply rninj, nfrle, nax_hd.
 Qed.
 
-Lemma frl_nfree : forall A x, ~ In x (ffreevars A) -> rprove (A :: nil) (frl x A).
+Lemma frl_nfree : forall A x, ~ x ∈ A -> rprove (A :: nil) (frl x A).
 Proof. intros A x Hnf; rev_intros; rnow rewrite nfree_subs. Qed.
 
 Lemma Kcombi : forall A B, rprove nil (imp A (imp B A)).
@@ -1132,5 +685,5 @@ apply (nimpe B).
   auto_nax.
 Qed.
 
-End Formulas.
+End Proofs.
 
